<?xml version="1.0"?>
<rdf:RDF xmlns="https://w3id.org/AlmesCore#"
     xml:base="https://w3id.org/AlmesCore"
     xmlns:dcat="https://www.w3.org/ns/dcat#"
     xmlns:dct="http://purl.org/dc/terms/"
     xmlns:dc="http://purl.org/dc/elements/1.1/"
     xmlns:alm="https://w3id.org/AlmesCore#"
     xmlns:foaf="http://xmlns.com/foaf/0.1/"
     xmlns:sdo="https://schema.org/"
     xmlns:gn="http://www.geonames.org/ontology#"
     xmlns:xsd="http://www.w3.org/2001/XMLSchema#"
     xmlns:rdfs="http://www.w3.org/2000/01/rdf-schema#"
     xmlns:owl="http://www.w3.org/2002/07/owl#"
     xmlns:rdf="http://www.w3.org/1999/02/22-rdf-syntax-ns#">

    <!-- Ontology Definition -->
    <owl:Ontology rdf:about="https://w3id.org/AlmesCore">
    <dcterms:title xml:lang="en">Agriculture and Livestock Metadata Elements Set (Almes Core)</dcterms:title>
    <dcterms:description xml:lang="en">
        This document presents the latest version of the Agriculture and Livestock Metadata Element Set (Almes Core),
        curated by the Almes Core Data Management Group. It encompasses comprehensive definitions of classes,
        properties, vocabulary encoding schemes, and syntax encoding schemes. The current core focuses on
        providing a detailed description of agricultural price index datasets.
    </dcterms:description>
    
    <!-- Version Information -->
    <owl:versionInfo>2.0.1</owl:versionInfo>
    <dcterms:issued rdf:datatype="http://www.w3.org/2001/XMLSchema#date">2024-10-15</dcterms:issued>
    <dcterms:modified rdf:datatype="http://www.w3.org/2001/XMLSchema#date">2024-10-15</dcterms:modified>
    
    <!-- Creator -->
    <dcterms:creator>
        <foaf:Organization>
            <foaf:name>Almes Core Management Group</foaf:name>
        </foaf:Organization>
    </dcterms:creator>
    
    <!-- Contributors -->
    <dcterms:contributor>
        <foaf:Person rdf:about="https://orcid.org/0000-0002-0674-7960">
            <foaf:name>Filipi Miranda Soares</foaf:name>
        </foaf:Person>
    </dcterms:contributor>
    <dcterms:contributor>
        <foaf:Person rdf:about="https://orcid.org/0000-0002-2744-6104">
            <foaf:name>Fernando Elias Corrêa</foaf:name>
        </foaf:Person>
    </dcterms:contributor>
    <dcterms:contributor>
        <foaf:Person rdf:about="https://orcid.org/0000-0002-4801-2225">
            <foaf:name>Dilvan de Abreu Moreira</foaf:name>
        </foaf:Person>
    </dcterms:contributor>
    <dcterms:contributor>
        <foaf:Person rdf:about="https://orcid.org/0000-0003-4177-1322">
            <foaf:name>Debora Pignatari Drucker</foaf:name>
        </foaf:Person>
    </dcterms:contributor>
    <dcterms:contributor>
        <foaf:Person rdf:about="https://orcid.org/0000-0001-6218-6849">
            <foaf:name>Kelly Rosa Braghetto</foaf:name>
        </foaf:Person>
    </dcterms:contributor>
    <dcterms:contributor>
        <foaf:Person rdf:about="https://orcid.org/0000-0003-1810-1742">
            <foaf:name>Alexandre Cláudio Botazzo Delbem</foaf:name>
        </foaf:Person>
    </dcterms:contributor>
    <dcterms:contributor>
        <foaf:Person rdf:about="https://orcid.org/0000-0001-7432-7653">
            <foaf:name>Luís Ferreira Pires</foaf:name>
        </foaf:Person>
    </dcterms:contributor>
    <dcterms:contributor>
        <foaf:Person rdf:about="https://orcid.org/0000-0002-1164-1351">
            <foaf:name>Luiz Olavo Bonino da Silva Santos</foaf:name>
        </foaf:Person>
    </dcterms:contributor>
    <dcterms:contributor>
        <foaf:Person rdf:about="https://orcid.org/0000-0003-2283-1123">
            <foaf:name>Antonio Mauro Saraiva</foaf:name>
        </foaf:Person>
    </dcterms:contributor>
    
    <!-- License -->
    <dcterms:license rdf:resource="https://creativecommons.org/licenses/by/4.0/" />
    
    <!-- Keywords -->
    <dcterms:subject>Agriculture</dcterms:subject>
    <dcterms:subject>Metadata Schema</dcterms:subject>
    <dcterms:subject>Commodities</dcterms:subject>
    <dcterms:subject>Price Index</dcterms:subject>
    
    <!-- Download Links -->
    <dcat:distribution>
        <dcat:Distribution>
            <dcat:accessURL rdf:resource="https://github.com/AlmesCore/Almes-Core/blob/main/core2024-07-08.md#almes-core-reference-guide"/>
            <dcterms:format>text/html</dcterms:format>
        </dcat:Distribution>
    </dcat:distribution>
    <dcat:distribution>
        <dcat:Distribution>
            <dcat:accessURL rdf:resource="https://raw.githubusercontent.com/AlmesCore/Almes-Core/refs/heads/main/Serializations/almes-core-schema-shacl.ttl"/>
            <dcterms:format>text/turtle</dcterms:format>
        </dcat:Distribution>
    </dcat:distribution>
    <dcat:distribution>
        <dcat:Distribution>
            <dcat:accessURL rdf:resource="https://raw.githubusercontent.com/AlmesCore/Almes-Core/refs/heads/main/Serializations/almes-core-schema.json"/>
            <dcterms:format>application/ld+json</dcterms:format>
        </dcat:Distribution>
    </dcat:distribution>
    <dcat:distribution>
        <dcat:Distribution>
            <dcat:accessURL rdf:resource="https://raw.githubusercontent.com/AlmesCore/Almes-Core/refs/heads/main/Serializations/almes-core-schema.plantuml"/>
            <dcterms:format>application/plantuml</dcterms:format>
        </dcat:Distribution>
    </dcat:distribution>

    <!-- Version History -->
    <dcterms:hasPart>
        <dcterms:BibliographicResource>
            <dcterms:title>Version History</dcterms:title>
            <dcterms:hasVersion rdf:resource="https://github.com/AlmesCore/Almes-Core/blob/main/deprecatedElements.md"/>
        </dcterms:BibliographicResource>
    </dcterms:hasPart>

    </owl:Ontology>

    <owl:Class rdf:about="dcat:Resource">
        <rdfs:label xml:lang="en">Resource</rdfs:label>
        <rdfs:label xml:lang="pt-br">Recurso</rdfs:label>
        <rdfs:comment xml:lang="en">Resource published or curated by a single agent.</rdfs:comment>
    </owl:Class>

    <owl:Class rdf:about="dcat:Dataset">
        <rdfs:label xml:lang="en">Dataset</rdfs:label>
        <rdfs:label xml:lang="pt-br">Dataset</rdfs:label>
        <rdfs:comment xml:lang="en">Data encoded in a defined structure.</rdfs:comment>
    </owl:Class>

    <owl:Class rdf:about="foaf:Agent">
        <rdfs:label xml:lang="en">Agent</rdfs:label>
        <rdfs:label xml:lang="pt-br">Agente</rdfs:label>
        <rdfs:comment xml:lang="en">An agent (e.g., person, group, software, or physical artifact).</rdfs:comment>
    </owl:Class>

    <owl:Class rdf:about="gn:Feature">
        <rdfs:label xml:lang="en">GeoNames Feature</rdfs:label>
        <rdfs:label xml:lang="pt-br">Característica Geográfica</rdfs:label>
        <rdfs:comment xml:lang="en">A geographical feature. It can be any feature that has a geographical extent, such as a country, city, mountain, river, etc.</rdfs:comment>
    </owl:Class>

    <owl:Class rdf:about="alm:Observation">
        <rdfs:label xml:lang="en">Observation</rdfs:label>
        <rdfs:label xml:lang="pt-br">Observação</rdfs:label>
        <rdfs:comment xml:lang="en">A recorded observation of an agricultural product price on a specific date. The observation captures key attributes such as the price, date of observation, and the applicable currency, which provide a snapshot of the economic value of the product at a given time.</rdfs:comment>
    </owl:Class>

    <owl:DatatypeProperty rdf:about="dct:identifier">
        <rdfs:label xml:lang="en">identifier</rdfs:label>
        <rdfs:label xml:lang="pt-br">identificador</rdfs:label>
        <rdfs:comment xml:lang="en">An unambiguous reference to the resource within a given context.</rdfs:comment>
        <rdfs:domain rdf:resource="dcat:Resource"/>
        <rdfs:range rdf:resource="xsd:anyURI"/>
    </owl:DatatypeProperty>

    <owl:DatatypeProperty rdf:about="dc:title">
        <rdfs:label xml:lang="en">title</rdfs:label>
        <rdfs:label xml:lang="pt-br">título</rdfs:label>
        <rdfs:comment xml:lang="en">A name given to the resource.</rdfs:comment>
        <rdfs:domain rdf:resource="dcat:Resource"/>
        <rdfs:range rdf:resource="rdfs:Literal"/>
    </owl:DatatypeProperty>

    <owl:DatatypeProperty rdf:about="dct:description">
        <rdfs:label xml:lang="en">description</rdfs:label>
        <rdfs:label xml:lang="pt-br">descrição</rdfs:label>
        <rdfs:comment xml:lang="en">An abstract, table of contents, a graphical representation, or a free-text account of the resource.</rdfs:comment>
        <rdfs:domain rdf:resource="dcat:Resource"/>
        <rdfs:range rdf:resource="rdfs:Literal"/>
    </owl:DatatypeProperty>

    <owl:DatatypeProperty rdf:about="dc:publisher">
        <rdfs:label xml:lang="en">publisher</rdfs:label>
        <rdfs:label xml:lang="pt-br">editor</rdfs:label>
        <rdfs:comment xml:lang="en">An entity responsible for making the resource available.</rdfs:comment>
        <rdfs:domain rdf:resource="dcat:Resource"/>
        <rdfs:range rdf:resource="foaf:Agent"/>
    </owl:DatatypeProperty>

    <owl:DatatypeProperty rdf:about="dc:creator">
        <rdfs:label xml:lang="en">creator</rdfs:label>
        <rdfs:label xml:lang="pt-br">criador</rdfs:label>
        <rdfs:comment xml:lang="en">An entity primarily responsible for making the resource.</rdfs:comment>
        <rdfs:domain rdf:resource="dcat:Resource"/>
        <rdfs:range rdf:resource="foaf:Agent"/>
    </owl:DatatypeProperty>

    <owl:DatatypeProperty rdf:about="dct:modified">
        <rdfs:label xml:lang="en">modified</rdfs:label>
        <rdfs:label xml:lang="pt-br">última atualização</rdfs:label>
        <rdfs:comment xml:lang="en">Date on which the resource was changed.</rdfs:comment>
        <rdfs:domain rdf:resource="dcat:Resource"/>
        <rdfs:range rdf:resource="xsd:date"/>
    </owl:DatatypeProperty>

    <owl:DatatypeProperty rdf:about="dct:hasVersion">
        <rdfs:label xml:lang="en">version</rdfs:label>
        <rdfs:label xml:lang="pt-br">versão</rdfs:label>
        <rdfs:comment xml:lang="en">The version indicator (name or identifier) of a resource.</rdfs:comment>
        <rdfs:domain rdf:resource="dcat:Resource"/>
        <rdfs:range rdf:resource="rdfs:Literal"/>
    </owl:DatatypeProperty>

    <owl:DatatypeProperty rdf:about="dct:language">
        <rdfs:label xml:lang="en">language</rdfs:label>
        <rdfs:label xml:lang="pt-br">idioma</rdfs:label>
        <rdfs:comment xml:lang="en">A language of the resource.</rdfs:comment>
        <rdfs:domain rdf:resource="dcat:Resource"/>
        <rdfs:range rdf:resource="rdfs:Literal"/>
    </owl:DatatypeProperty>

    <owl:DatatypeProperty rdf:about="dct:license">
        <rdfs:label xml:lang="en">license</rdfs:label>
        <rdfs:label xml:lang="pt-br">licença de uso</rdfs:label>
        <rdfs:comment xml:lang="en">A legal document giving official permission to do something with the resource.</rdfs:comment>
        <rdfs:domain rdf:resource="dcat:Resource"/>
        <rdfs:range rdf:resource="xsd:anyURI"/>
    </owl:DatatypeProperty>

    <owl:DatatypeProperty rdf:about="dc:rights">
        <rdfs:label xml:lang="en">rights</rdfs:label>
        <rdfs:label xml:lang="pt-br">direitos</rdfs:label>
        <rdfs:comment xml:lang="en">Information about rights held in and over the resource.</rdfs:comment>
        <rdfs:domain rdf:resource="dcat:Resource"/>
        <rdfs:range rdf:resource="rdfs:Literal"/>
    </owl:DatatypeProperty>

    <owl:DatatypeProperty rdf:about="alm:productgroup">
        <rdfs:label xml:lang="en">product group</rdfs:label>
        <rdfs:label xml:lang="pt-br">grupo do produto</rdfs:label>
        <rdfs:comment xml:lang="en">A ProductGroup represents a group of products resulting from agriculture or livestock activities that vary only in certain well-described ways.</rdfs:comment>
        <rdfs:domain rdf:resource="dcat:Dataset"/>
        <rdfs:range rdf:resource="rdfs:Literal"/>
    </owl:DatatypeProperty>

    <owl:DatatypeProperty rdf:about="alm:productgroupuri">
        <rdfs:label xml:lang="en">product group URI</rdfs:label>
        <rdfs:label xml:lang="pt-br">URI do grupo do produto</rdfs:label>
        <rdfs:comment xml:lang="en">A URI of a term from any controlled vocabulary describing a productGroup.</rdfs:comment>
        <rdfs:domain rdf:resource="dcat:Dataset"/>
        <rdfs:range rdf:resource="xsd:anyURI"/>
    </owl:DatatypeProperty>

    <owl:DatatypeProperty rdf:about="alm:productgroupname">
        <rdfs:label xml:lang="en">product group name</rdfs:label>
        <rdfs:label xml:lang="pt-br">nome do grupo do produto</rdfs:label>
        <rdfs:comment xml:lang="en">The name of a productGroup in a controlled vocabulary.</rdfs:comment>
        <rdfs:domain rdf:resource="dcat:Dataset"/>
        <rdfs:range rdf:resource="rdfs:Literal"/>
    </owl:DatatypeProperty>

    <owl:DatatypeProperty rdf:about="alm:producttype">
        <rdfs:label xml:lang="en">product type</rdfs:label>
        <rdfs:label xml:lang="pt-br">produto</rdfs:label>
        <rdfs:comment xml:lang="en">Name of the agricultural or livestock product type targeted by the commercial operation.</rdfs:comment>
        <rdfs:domain rdf:resource="dcat:Dataset"/>
        <rdfs:range rdf:resource="rdfs:Literal"/>
    </owl:DatatypeProperty>

    <owl:DatatypeProperty rdf:about="alm:producttypeuri">
        <rdfs:label xml:lang="en">product type URI</rdfs:label>
        <rdfs:label xml:lang="pt-br">URI do tipo de produto</rdfs:label>
        <rdfs:comment xml:lang="en">A URI of a term from any controlled vocabulary describing a productType.</rdfs:comment>
        <rdfs:domain rdf:resource="dcat:Dataset"/>
        <rdfs:range rdf:resource="xsd:anyURI"/>
    </owl:DatatypeProperty>

    <owl:DatatypeProperty rdf:about="alm:producttypename">
        <rdfs:label xml:lang="en">product type name</rdfs:label>
        <rdfs:label xml:lang="pt-br">nome do tipo de produto</rdfs:label>
        <rdfs:comment xml:lang="en">The name of a productType in a controlled vocabulary.</rdfs:comment>
        <rdfs:domain rdf:resource="dcat:Dataset"/>
        <rdfs:range rdf:resource="rdfs:Literal"/>
    </owl:DatatypeProperty>

    <owl:DatatypeProperty rdf:about="alm:theme">
        <rdfs:label xml:lang="en">theme</rdfs:label>
        <rdfs:label xml:lang="pt-br">tema</rdfs:label>
        <rdfs:comment xml:lang="en">Indicates the main subject or topic investigated in the economic statistical operation.</rdfs:comment>
        <rdfs:domain rdf:resource="dcat:Dataset"/>
        <rdfs:range rdf:resource="rdfs:Literal"/>
    </owl:DatatypeProperty>

    <owl:DatatypeProperty rdf:about="dcat:accessURL">
        <rdfs:label xml:lang="en">access URL</rdfs:label>
        <rdfs:label xml:lang="pt-br">disponível em</rdfs:label>
        <rdfs:comment xml:lang="en">A URL of the resource that gives access to a distribution of the dataset.</rdfs:comment>
        <rdfs:domain rdf:resource="dcat:Dataset"/>
        <rdfs:range rdf:resource="xsd:anyURI"/>
    </owl:DatatypeProperty>

    <owl:DatatypeProperty rdf:about="dct:accrualPeriodicity">
        <rdfs:label xml:lang="en">periodicity</rdfs:label>
        <rdfs:label xml:lang="pt-br">periodicidade</rdfs:label>
        <rdfs:comment xml:lang="en">The frequency with which items are added to a collection.</rdfs:comment>
        <rdfs:domain rdf:resource="dcat:Dataset"/>
        <rdfs:range rdf:resource="rdfs:Literal"/>
    </owl:DatatypeProperty>

    <owl:DatatypeProperty rdf:about="sdo:referenceQuantity">
        <rdfs:label xml:lang="en">reference quantity</rdfs:label>
        <rdfs:label xml:lang="pt-br">quantidade de referência</rdfs:label>
        <rdfs:comment xml:lang="en">The reference quantity for which a certain price applies.</rdfs:comment>
        <rdfs:domain rdf:resource="dcat:Dataset"/>
        <rdfs:range rdf:resource="rdfs:Literal"/>
    </owl:DatatypeProperty>

    <owl:DatatypeProperty rdf:about="sdo:location">
        <rdfs:label xml:lang="en">location</rdfs:label>
        <rdfs:label xml:lang="pt-br">localização</rdfs:label>
        <rdfs:comment xml:lang="en">The location of, for example, where an event is happening or where an action takes place.</rdfs:comment>
        <rdfs:domain rdf:resource="dcat:Dataset"/>
        <rdfs:range rdf:resource="gn:Feature"/>
    </owl:DatatypeProperty>

    <owl:DatatypeProperty rdf:about="alm:statisticalMethod">
        <rdfs:label xml:lang="en">statistical method</rdfs:label>
        <rdfs:label xml:lang="pt-br">método estatístico</rdfs:label>
        <rdfs:comment xml:lang="en">Summary of the methods used for the process of obtaining data.</rdfs:comment>
        <rdfs:domain rdf:resource="dcat:Dataset"/>
        <rdfs:range rdf:resource="xsd:anyURI"/>
    </owl:DatatypeProperty>

    <owl:DatatypeProperty rdf:about="alm:descriptiveStatistics">
        <rdfs:label xml:lang="en">descriptive statistics</rdfs:label>
        <rdfs:label xml:lang="pt-br">estatística descritiva</rdfs:label>
        <rdfs:comment xml:lang="en">Summarizes and describes the main features of a dataset.</rdfs:comment>
        <rdfs:domain rdf:resource="dcat:Dataset"/>
        <rdfs:range rdf:resource="rdfs:Literal"/>
    </owl:DatatypeProperty>

    <owl:DatatypeProperty rdf:about="sdo:startDate">
        <rdfs:label xml:lang="en">start date</rdfs:label>
        <rdfs:label xml:lang="pt-br">data de início</rdfs:label>
        <rdfs:comment xml:lang="en">The start date and time of the item (in ISO 8601 date format).</rdfs:comment>
        <rdfs:domain rdf:resource="dcat:Dataset"/>
        <rdfs:range rdf:resource="xsd:date"/>
    </owl:DatatypeProperty>

    <owl:DatatypeProperty rdf:about="sdo:endDate">
        <rdfs:label xml:lang="en">end date</rdfs:label>
        <rdfs:label xml:lang="pt-br">data de fim</rdfs:label>
        <rdfs:comment xml:lang="en">The end date and time of the item (in ISO 8601 date format).</rdfs:comment>
        <rdfs:domain rdf:resource="dcat:Dataset"/>
        <rdfs:range rdf:resource="xsd:date"/>
    </owl:DatatypeProperty>

    <owl:DatatypeProperty rdf:about="alm:hasObservation">
        <rdfs:label xml:lang="en">has observation</rdfs:label>
        <rdfs:label xml:lang="pt-br">tem observação</rdfs:label>
        <rdfs:comment xml:lang="en">Associates an entity to a specific recorded price Observation related to an agricultural product.</rdfs:comment>
        <rdfs:domain rdf:resource="dcat:Dataset"/>
        <rdfs:range rdf:resource="alm:Observation"/>
    </owl:DatatypeProperty>

    <owl:DatatypeProperty rdf:about="foaf:name">
        <rdfs:label xml:lang="en">name</rdfs:label>
        <rdfs:label xml:lang="pt-br">nome</rdfs:label>
        <rdfs:comment xml:lang="en">A name for some thing.</rdfs:comment>
        <rdfs:domain rdf:resource="foaf:Agent"/>
        <rdfs:range rdf:resource="rdfs:Literal"/>
    </owl:DatatypeProperty>

    <owl:DatatypeProperty rdf:about="foaf:homepage">
        <rdfs:label xml:lang="en">homepage</rdfs:label>
        <rdfs:label xml:lang="pt-br">homepage</rdfs:label>
        <rdfs:comment xml:lang="en">A homepage for some thing.</rdfs:comment>
        <rdfs:domain rdf:resource="foaf:Agent"/>
        <rdfs:range rdf:resource="xsd:anyURI"/>
    </owl:DatatypeProperty>

    <owl:DatatypeProperty rdf:about="foaf:mbox">
        <rdfs:label xml:lang="en">e-mail</rdfs:label>
        <rdfs:label xml:lang="pt-br">e-mail</rdfs:label>
        <rdfs:comment xml:lang="en">A personal mailbox, associated with exactly one owner. This is a 'static inverse functional property'.</rdfs:comment>
        <rdfs:domain rdf:resource="foaf:Agent"/>
        <rdfs:range rdf:resource="rdfs:Literal"/>
    </owl:DatatypeProperty>

    <owl:DatatypeProperty rdf:about="gn:name">
        <rdfs:label xml:lang="en">geoNames name</rdfs:label>
        <rdfs:label xml:lang="pt-br">nome geoNames</rdfs:label>
        <rdfs:comment xml:lang="en">The name of a geographical feature. Examples: New York, Mount Everest, Nile River.</rdfs:comment>
        <rdfs:domain rdf:resource="gn:Feature"/>
        <rdfs:range rdf:resource="rdfs:Literal"/>
    </owl:DatatypeProperty>

    <owl:DatatypeProperty rdf:about="gn:geonamesID">
        <rdfs:label xml:lang="en">geonames ID</rdfs:label>
        <rdfs:label xml:lang="pt-br">identificador geoNames</rdfs:label>
        <rdfs:comment xml:lang="en">The ID of a geographical feature. Examples: http://sws.geonames.org/5128581/, http://sws.geonames.org/6252001/, http://sws.geonames.org/2347283/.</rdfs:comment>
        <rdfs:domain rdf:resource="gn:Feature"/>
        <rdfs:range rdf:resource="xsd:anyURI"/>
    </owl:DatatypeProperty>

    <owl:DatatypeProperty rdf:about="dc:date">
        <rdfs:label xml:lang="en">date</rdfs:label>
        <rdfs:label xml:lang="pt-br">data</rdfs:label>
        <rdfs:comment xml:lang="en">A point or period of time associated with an event in the lifecycle of the resource. Recommended practice is to express the date according to ISO 8601-1.</rdfs:comment>
        <rdfs:domain rdf:resource="alm:Observation"/>
        <rdfs:range rdf:resource="xsd:date"/>
    </owl:DatatypeProperty>

    <owl:DatatypeProperty rdf:about="sdo:price">
        <rdfs:label xml:lang="en">price</rdfs:label>
        <rdfs:label xml:lang="pt-br">preço</rdfs:label>
        <rdfs:comment xml:lang="en">The offer price of a product. The price should be indicated as a float number with two decimal digits.</rdfs:comment>
        <rdfs:domain rdf:resource="alm:Observation"/>
        <rdfs:range rdf:resource="xsd:float"/>
    </owl:DatatypeProperty>

    <owl:DatatypeProperty rdf:about="sdo:currency">
        <rdfs:label xml:lang="en">currency</rdfs:label>
        <rdfs:label xml:lang="pt-br">moeda</rdfs:label>
        <rdfs:comment xml:lang="en">The currency in which the monetary amount is expressed. Use standard formats: ISO 4217 currency format (e.g., USD), ticker symbols for cryptocurrencies (e.g., BTC), or well-known names for local exchange trading systems.</rdfs:comment>
        <rdfs:domain rdf:resource="alm:Observation"/>
        <rdfs:range rdf:resource="xsd:string"/>
    </owl:DatatypeProperty>

</rdf:RDF>
